Splinter/Betree/LinkedBetreeForest.i.dfy
@@ -1,0 +1,858 @@
+// Copyright 2018-2021 VMware, Inc., Microsoft Inc., Carnegie Mellon University, ETH Zurich, and University of Washington
+// SPDX-License-Identifier: BSD-2-Clause
+
+include "PivotBetree.i.dfy"
+include "../../lib/Buckets/BoundedPivotsLib.i.dfy"
+include "../Journal/GenericDisk.i.dfy"
+include "Domain.i.dfy"
+include "LinkedForest.i.dfy"
+
+// TODO:
+// This module deals with 
+// 1. Concretize buffer implementation with Forest (seqs of B+ tree)
+// 2. Filter should be implicitly tracked by pivot table (no more apply filters)
+//    - In LinkedBetree we did not restrict the range of splitted child
+// 3. Track active buffers for each child, as we don't want to visit a buffer that is flushed to a child already
+
+// Naming: BranchedBetree? 
+module LinkedBetreeForest
+{
+  import opened BoundedPivotsLib
+  import opened DomainMod
+  import opened GenericDisk
+  import opened KeyType
+  import opened LSNMod
+  import opened MemtableMod
+  import opened MsgHistoryMod
+  import opened Options
+  import opened Sequences
+  import opened StampedMod
+  import opened Upperbounded_Lexicographic_Byte_Order_Impl
+  import opened Upperbounded_Lexicographic_Byte_Order_Impl.Ord
+  import opened ValueMessage
+  import opened Maps
+  import TotalKMMapMod
+  
+  import LF = LinkedForestMod
+  import LB = LinkedBranchMod
+
+  type Pointer = GenericDisk.Pointer
+  type Address = GenericDisk.Address
+  type StampedBetree = Stamped<LinkedBetree>
+  type StampedForest = Stamped<LF.LinkedForest> // TODO: revisit after marshall layer 
+
+  function EmptyLinkedBetree() : (out: LinkedBetree)
+  {
+    LinkedBetree(None, EmptyDisk())
+  }
+
+  function EmptyImage() : StampedBetree
+  {
+    Stamped(EmptyLinkedBetree(), 0)
+  }
+
+  type Element = Upperbounded_Lexicographic_Byte_Order_Impl.Ord.Element
+
+  datatype TransitionLabel =
+      QueryLabel(endLsn: LSN, key: Key, value: Value)
+    | PutLabel(puts: MsgHistory)
+    | QueryEndLsnLabel(endLsn: LSN)
+    | FreezeAsLabel(linkedBetree: StampedBetree, forest: StampedForest)
+    | InternalLabel()
+
+
+  datatype BetreeNode = BetreeNode(
+    // bundle's filter apply to multiple branches
+    buffers: seq<Address>, // Forest Disk
+    pivotTable: PivotTable,
+    children: seq<Pointer>, // Betree Disk
+    activeBufferRanges: seq<nat>  // parallel DS to children array, each entry stores the start of active buffer range for the corresponding child
+  ) {
+    predicate WF() {
+      && WFPivots(pivotTable)
+      && |children| == NumBuckets(pivotTable)
+      && |children| == |activeBufferRanges|
+      && (forall i | i < |activeBufferRanges| :: activeBufferRanges[i] <= |buffers|)
+    }
+
+    // predicate 
+
+    predicate ValidChildIndex(childIdx: nat)
+    {
+      && BetreeNode?
+      && childIdx < NumBuckets(pivotTable)
+    }
+
+    predicate OccupiedChildIndex(childIdx: nat)
+      requires WF()
+    {
+      && ValidChildIndex(childIdx)
+      && children[childIdx].Some?
+    }
+
+    function PushBufferStack(addr: Address) : (out: BetreeNode)
+      requires WF()
+      ensures out.WF()
+    {
+      BetreeNode(buffers + [addr], pivotTable, children, activeBufferRanges)
+    }
+
+    // TODO: doesn't belong here anymore because we can no longer just reach into things now
+    // function ApplyFilter(filter: Domain) : (out: BetreeNode)
+    //   requires WF()
+    //   ensures out.WF()
+    // {
+    //   BetreeNode(buffers.ApplyFilter(filter.KeySet()), pivotTable, children)
+    // }
+
+    function ChildDomain(childIdx: nat) : (out: Domain)
+      requires WF()
+      requires BetreeNode?
+      requires ValidChildIndex(childIdx)
+      ensures out.WF()
+    {
+      var out := Domain(pivotTable[childIdx], pivotTable[childIdx+1]);
+      reveal_IsStrictlySorted();
+      out.reveal_SaneKeys(); 
+      out
+    }
+
+    predicate KeyInDomain(key: Key)
+    {
+      && WF()
+      && BetreeNode?
+      && BoundedKey(pivotTable, key)
+    }
+
+    function ChildPtr(key: Key) : Pointer
+      requires KeyInDomain(key)
+    {
+      children[Route(pivotTable, key)]
+    }
+
+    function ChildBufferRange(key: Key) : (i: nat)
+      requires KeyInDomain(key)
+    {
+      activeBufferRanges[Route(pivotTable, key)]
+    }
+  }
+
+  // PivotTable constructor for a total domain
+  function TotalPivotTable() : PivotTable
+  {
+    [TotalDomain().start, TotalDomain().end]
+  }
+
+  // BetreeNode constructor for empty node
+  function EmptyRoot(domain: Domain) : (out: BetreeNode)
+    requires domain.WF()
+    requires domain.Domain?
+    ensures out.WF()
+  {
+    var pivotTable := [domain.start, domain.end];
+    domain.reveal_SaneKeys();  /* jonh suspicious lt leak */
+    assert Keyspace.IsStrictlySorted(pivotTable) by { reveal_IsStrictlySorted(); }  /* jonh suspicious lt leak */
+    BetreeNode([], pivotTable, [None], [0])
+  }
+
+  datatype DiskView = DiskView(entries: map<Address, BetreeNode>) 
+  {
+    // TODO(jonh): some duplication with LinkedJournal.DiskView; refactor into library superclassish thing?
+    // Or a generic with GenericDisk.DiskView<T>?
+    // BetreeNodes are WF()
+    predicate EntriesWF() 
+    {
+      (forall addr | addr in entries :: entries[addr].WF())
+    }
+
+    predicate IsNondanglingPointer(ptr: Pointer)
+    {
+      ptr.Some? ==> ptr.value in entries
+    }
+
+    predicate NodeHasNondanglingChildPtrs(node: BetreeNode)
+    {
+      node.BetreeNode? ==>
+      (forall idx:nat | idx < |node.children| :: IsNondanglingPointer(node.children[idx]))
+    }
+
+    predicate NoDanglingPointers()  // i.e. disk is closed wrt to all the pointers in the nodes on disk
+    {
+      (forall addr | addr in entries :: NodeHasNondanglingChildPtrs(entries[addr]))
+    }
+
+    predicate WF()
+    {
+      && EntriesWF()
+      && NoDanglingPointers()
+    }   
+
+    function Get(ptr: Pointer) : BetreeNode
+      // requires WF()
+      requires IsNondanglingPointer(ptr)
+      requires ptr.Some?
+    {
+      entries[ptr.value]
+    }
+
+    // buffer not in entries, it belongs to a different disk
+    predicate BufferInNode(buffer: Address)
+    {
+      (exists addr :: addr in entries && entries[addr].BetreeNode? && buffer in entries[addr].buffers)
+    }
+
+    function Buffers() : iset<Address>
+    {
+      iset buffer:Address | BufferInNode(buffer)
+    }
+
+    predicate AgreesWithDisk(other: DiskView)
+    {
+      MapsAgree(entries, other.entries)
+    }
+
+    predicate IsSubsetOf(other: DiskView)
+    {
+      && entries.Keys <= other.entries.Keys 
+      && AgreesWithDisk(other)
+    }
+
+    // The node at this address has child pointers that respect ranking
+    predicate NodeChildrenRespectsRank(ranking: Ranking, addr: Address)
+      requires WF()
+      requires addr in entries
+      requires addr in ranking
+    {
+      && var node := entries[addr];
+      && (forall childIdx:nat | node.ValidChildIndex(childIdx) && node.children[childIdx].Some? ::
+        && node.children[childIdx].value in ranking  // ranking is closed
+        && ranking[node.children[childIdx].value] < ranking[addr]  // decreases
+      )
+    }
+
+    // Together with NodeChildrenRespectsRank, this says that ranking is closed
+    predicate ValidRanking(ranking: Ranking) 
+      requires WF()
+    {
+      forall addr | 
+        && addr in ranking 
+        && addr in entries 
+      ::
+        NodeChildrenRespectsRank(ranking, addr)
+    }
+
+    predicate IsFresh(addrs: set<Address>) {
+      addrs !! entries.Keys
+    } 
+
+    function {:opaque} MergeDisk(other: DiskView) : (out: DiskView)
+      // ensure result is sound -- keys and their values must come from one of these places
+      ensures forall addr | addr in out.entries 
+        :: || (addr in entries && out.entries[addr] == entries[addr])
+           || (addr in other.entries && out.entries[addr] == other.entries[addr])
+      // ensure result is complete -- result must contain all the keys
+      ensures entries.Keys <= out.entries.Keys
+      ensures other.entries.Keys <= out.entries.Keys
+    {
+      DiskView.DiskView(MapUnion(entries, other.entries))
+    }
+  }
+
+  function EmptyDisk() : DiskView {
+    DiskView.DiskView(map[])
+  }
+
+  function {:opaque} MergeDiskViews(diskViews: seq<DiskView>) : (out: DiskView)
+    // ensure result is sound -- keys and their values must come from one of these places
+    ensures forall addr | addr in out.entries 
+      :: (exists i :: 
+            && 0 <= i < |diskViews|
+            && addr in diskViews[i].entries
+            && out.entries[addr] == diskViews[i].entries[addr]
+      )
+    // ensure result is complete -- result must contain all the keys
+    ensures forall i | 0 <= i < |diskViews| :: diskViews[i].entries.Keys <= out.entries.Keys
+    decreases |diskViews|
+  { var out :=
+      if |diskViews| == 0 then EmptyDisk()
+      else diskViews[0].MergeDisk(MergeDiskViews(diskViews[1..]));
+    reveal_MergeDiskViews();
+    out
+  }
+
+  
+  // This is the unit of interpretation: A LinkedBetree has enough info in it to interpret to a PivotBetree.BetreeNode.
+  datatype LinkedBetree = LinkedBetree(
+    root: Pointer,
+    diskView: DiskView
+  )
+  {
+    predicate WF() {
+      && diskView.WF()
+      && diskView.IsNondanglingPointer(root)
+    }
+
+    predicate HasRoot() {
+      && diskView.IsNondanglingPointer(root)
+      && root.Some?
+    }
+
+    function Root() : BetreeNode
+      requires HasRoot()
+    {
+      diskView.Get(root)
+    }
+
+    function ChildAtIdx(idx: nat) : LinkedBetree
+      requires WF()
+      requires HasRoot()
+      requires Root().ValidChildIndex(idx)
+    {
+      LinkedBetree(Root().children[idx], diskView)
+    }
+
+    function ChildForKey(key: Key) : LinkedBetree
+      requires HasRoot()
+      requires Root().KeyInDomain(key)
+    {
+      LinkedBetree(Root().ChildPtr(key), diskView)
+    }
+
+    function GetRank(ranking: Ranking) : nat
+      requires WF()
+    {
+      if HasRoot() && root.value in ranking then ranking[root.value]+1 else 0
+    }
+
+    function GetChildCount() : nat 
+      requires WF()
+    {
+      if HasRoot() then |Root().children| else 0
+    }
+
+    // this says that ranking is closed 
+    predicate ValidRanking(ranking: Ranking) 
+      requires WF()
+    {
+      && diskView.ValidRanking(ranking)
+      && (HasRoot() ==> root.value in ranking)  // ranking covers tree from this root
+    }
+
+    predicate Acyclic()
+    {
+      && WF()
+      && (exists ranking :: ValidRanking(ranking))
+    }
+
+    function TheRanking() : Ranking
+      requires Acyclic()
+    {
+      var out :| ValidRanking(out);
+      out
+    }
+
+    // Build a tight disk with respect to this root
+    function BuildTightTreeUsingRanking(ranking: Ranking) : (out: LinkedBetree)
+      requires WF()
+      requires ValidRanking(ranking)
+      ensures out.root == root
+      ensures HasRoot() ==> root.value in out.diskView.entries
+      ensures HasRoot() ==> out.diskView.entries[root.value] == Root()
+      decreases GetRank(ranking)
+    {
+      if !HasRoot()
+      then 
+        // base case, return empty disk
+        LinkedBetree(root, EmptyDisk())
+      else 
+        var numChildren := |Root().children|;
+        // list of tight diskviews at each of my children
+        var tightChildrenDvs := seq(numChildren, i requires 0 <= i < numChildren => ChildAtIdx(i).BuildTightTreeUsingRanking(ranking).diskView);
+        var dv := DiskView.DiskView(MergeDiskViews(tightChildrenDvs).entries[root.value := Root()]);
+        LinkedBetree(root, dv)
+    }
+    
+    function BuildTightTree() : LinkedBetree {
+      if Acyclic() then BuildTightTreeUsingRanking(TheRanking()) 
+      else this  // Can't build a tight tree if I'm not acyclic
+    }
+  }
+
+  
+  // LinkedBetreee w/ Forest State Machine
+
+  datatype Variables = Variables(
+    memtable: Memtable,
+    linked: LinkedBetree,
+    forestSM: LF.Variables)
+  {
+    // linked diskView and forest diskView should have disjoint addresses
+    predicate DisjointForest() {
+      && linked.diskView.IsFresh(forestSM.Addresses())
+    }
+
+    // buffers in each node should be known to forest
+    predicate BoundedForest() {
+      // && (forall addr, buffer | )
+      && (forall buffer | buffer in linked.diskView.Buffers() :: buffer in forestSM.forest.trees)
+    }
+
+    predicate WF() {
+      && linked.WF()
+      && forestSM.WF()
+      // TODO: move to Valid
+      && DisjointForest()
+      && BoundedForest()
+    }
+  }
+
+  // TODO(jonh): SO much copypasta from PivotBetree! Library, paramaterize child mechanism?
+  datatype QueryReceiptLine = QueryReceiptLine(
+    ptr: Pointer,
+    result: Message)
+  {
+    predicate WF()
+    {
+      && result.Define?
+    }
+  }
+
+  datatype QueryReceipt = QueryReceipt(
+    key: Key,
+    diskView: DiskView,
+    forest: LF.LinkedForest,
+    lines: seq<QueryReceiptLine>)
+  {
+    predicate Structure()
+    {
+      && 0 < |lines|
+      && (forall i:nat | i < |lines| :: lines[i].ptr.Some? <==> i < |lines|-1)
+      && (forall i:nat | i < |lines|-1 :: diskView.IsNondanglingPointer(lines[i].ptr))
+      && Last(lines).result == Define(DefaultValue())
+      && diskView.WF()
+      && forest.WF() // don't have to require disjointness here since query is read only 
+    }
+
+    function Node(i: nat) : (out:BetreeNode)
+      requires Structure()
+      requires i < |lines| - 1  // last line is None ptr
+      ensures out.WF()
+    {
+      diskView.Get(lines[i].ptr)
+    }
+
+    predicate AllLinesWF()
+    {
+      && Structure()
+      && (forall i:nat | i < |lines|-1 :: Node(i).KeyInDomain(key))
+      && (forall i:nat, buffer | i < |lines|-1 && buffer in Node(i).buffers :: forest.ValidTree(buffer))
+    }
+
+    predicate ChildLinkedAt(i: nat)
+      requires AllLinesWF()
+      requires i < |lines|-1
+    {
+      lines[i+1].ptr == Node(i).ChildPtr(key)
+    }
+
+    function ResultAt(i: nat) : Message
+      requires i < |lines|
+    {
+      lines[i].result
+    }
+
+    predicate ResultLinkedAt(i: nat)
+      requires Structure()
+      requires AllLinesWF()
+      requires i < |lines| - 1
+    {
+      && var start := Node(i).ChildBufferRange(key); // only query on a child's active range
+      && var msg := forest.Query(key, Node(i).buffers[start..]);
+      && lines[i].result == Merge(msg, ResultAt(i+1))
+    }
+
+    predicate Valid()
+    {
+      && Structure()
+      && AllLinesWF()
+      && (forall i:nat | i < |lines| - 1 :: ChildLinkedAt(i))
+      && (forall i:nat | i < |lines| - 1 :: ResultLinkedAt(i))
+    }
+
+    predicate ValidFor(linked: LinkedBetree, forest: LF.LinkedForest, key: Key)
+    {
+      && Valid()
+      && this.diskView == linked.diskView
+      && this.lines[0].ptr == linked.root
+      && this.forest == forest
+      && this.key == key
+    }
+
+    function Result() : Message
+      requires Structure()
+    {
+      ResultAt(0)
+    }
+  }
+
+  predicate Query(v: Variables, v': Variables, lbl: TransitionLabel, receipt: QueryReceipt)
+  {
+    && lbl.QueryLabel?
+    && lbl.endLsn == v.memtable.seqEnd
+    && receipt.ValidFor(v.linked, v.forestSM.forest, lbl.key)
+    && Define(lbl.value) == Merge(v.memtable.Query(lbl.key), receipt.Result())
+    && v' == v
+  }
+
+  predicate Put(v: Variables, v': Variables, lbl: TransitionLabel)
+  {
+    && lbl.PutLabel?
+    && lbl.puts.WF()
+    && lbl.puts.seqStart == v.memtable.seqEnd
+    && v' == v.(memtable := v.memtable.ApplyPuts(lbl.puts))
+  }
+
+  predicate QueryEndLsn(v: Variables, v': Variables, lbl: TransitionLabel)
+  {
+    && lbl.QueryEndLsnLabel?
+    && lbl.endLsn == v.memtable.seqEnd
+    && v' == v
+  }
+
+  predicate FreezeAs(v: Variables, v': Variables, lbl: TransitionLabel)
+  {
+    && lbl.FreezeAsLabel?
+    && v.WF()
+    && v.memtable.IsEmpty()
+    && lbl.linkedBetree == Stamped(v.linked, v.memtable.seqEnd)
+    && lbl.forest == Stamped(v.forestSM.forest, v.memtable.seqEnd) // TODO: revisit after marshall layer
+    && v' == v
+  }
+
+  predicate InternalFlushMemtable(v: Variables, v': Variables, lbl: TransitionLabel, step: Step)
+  {
+    && lbl.InternalLabel?
+    && step.InternalFlushMemtableStep?
+    && step.WF()
+    && assert step.branch.I().WF() by { step.branch.WFI( step.branch.I() ); } // TODO: revisit
+    && step.branch.I().I() == v.memtable.buffer  // new branch must represent memtable 
+
+    && v.WF()
+    && v'.WF() // be careful
+    && v'.linked.diskView.AgreesWithDisk(v.linked.diskView)
+      // NB: linked.WF() ==> No nondangling pointers, so in practice linked <= linked'
+    && v'.linked.HasRoot()
+    && v'.linked.Root() == (
+      if !v.linked.HasRoot()
+      then BetreeNode([step.branch.root], TotalPivotTable(), [None], [0])
+      else v.linked.Root().PushBufferStack(step.branch.root))
+
+    && LF.Next(v.forestSM, v'.forestSM, LF.AddTreeLabel(step.branch))
+  }
+
+  type PathAddrs = seq<Address>
+
+  // Question is should one of the restriction on path be that 
+  // replaced path can't have different, linked = a root (might even be a subtree and a disk)
+
+  datatype Path = Path(linked: LinkedBetree, key: Key, depth: nat)
+  {
+    function Subpath() : (out: Path)
+      requires 0 < depth
+      requires linked.HasRoot()
+      requires linked.Root().KeyInDomain(key)
+    {
+      Path(linked.ChildForKey(key), key, depth-1)
+    }
+
+    predicate Valid()
+      decreases depth
+    {
+      && linked.WF()
+      && linked.HasRoot()  
+      && linked.Root().KeyInDomain(key)
+      && (0 < depth ==> Subpath().Valid())  // implies path must lead to a non-nil node
+    }
+
+    function Target() : (out: LinkedBetree)
+      requires Valid()
+      ensures out.WF()
+      ensures out.root.Some?
+      ensures out.diskView == linked.diskView
+      ensures out.HasRoot() ==> out.root.value in out.diskView.entries
+      decreases depth
+    {
+      if 0 == depth
+      then linked
+      else Subpath().Target()
+    }
+
+    // shows that the Path can be replaced with 
+    // we want to maintain the same property with regard to forest as before
+    predicate CanSubstitute(replacement: LinkedBetree, pathAddrs: PathAddrs) 
+    {
+      && linked.WF()
+      && replacement.WF()
+      && depth == |pathAddrs|
+      && Valid()
+      && linked.diskView.IsSubsetOf(replacement.diskView)
+    }
+
+    function Substitute(replacement: LinkedBetree, pathAddrs: PathAddrs) : (out: LinkedBetree)
+      requires CanSubstitute(replacement, pathAddrs)
+      decreases depth, 1
+    { 
+      if depth == 0 
+      then replacement
+      else 
+        var node := linked.Root();
+        var subtree := Subpath().Substitute(replacement, pathAddrs[1..]);
+        var newChildren := node.children[Route(node.pivotTable, key) := subtree.root];
+        // child is replaced but no changes to buffers, so the new child should have the same 
+        // active buffer range as the old child 
+        var newNode := BetreeNode(node.buffers, node.pivotTable, newChildren, node.activeBufferRanges); 
+        var newDiskView := DiskView.DiskView(subtree.diskView.entries[pathAddrs[0] := newNode]); 
+        LinkedBetree(GenericDisk.Pointer.Some(pathAddrs[0]), newDiskView)
+    }
+  }
+
+  function InsertGrowReplacement(oldRoot: LinkedBetree, newRootAddr:Address) : (out: LinkedBetree)
+    requires oldRoot.WF()
+  {
+    // The new root node
+    var root' := BetreeNode([], TotalPivotTable(), [oldRoot.root], [0]);
+    // The new diskview
+    var dv' := DiskView.DiskView(oldRoot.diskView.entries[newRootAddr := root']); 
+    LinkedBetree(Pointer.Some(newRootAddr), dv')
+  } 
+
+  predicate InternalGrow(v: Variables, v': Variables, lbl: TransitionLabel, step: Step)
+  {
+    && v.WF()
+    && step.WF()
+    && lbl.InternalLabel?
+    && step.InternalGrowStep?
+    // Subway Eat Fresh!
+    && v.linked.diskView.IsFresh({step.newRootAddr})
+    && v' == v.(linked := InsertGrowReplacement(v.linked, step.newRootAddr).BuildTightTree())
+  }
+
+  predicate IsSplit(linked: LinkedBetree, linked': LinkedBetree, childIdx: nat, splitKey: Key)
+  {
+    && linked.WF()
+    && linked'.WF()
+    && linked.HasRoot()
+    && linked'.HasRoot()
+    && linked'.diskView.AgreesWithDisk(linked.diskView)
+    && var root := linked.Root();
+    && var root' := linked'.Root();
+
+    && root.ValidChildIndex(childIdx)
+    && PivotInsertable(root.pivotTable, childIdx, splitKey)
+    && 0 < childIdx < NumBuckets(root.pivotTable) // Split can't extend domain of this node.
+    && var oldChildPtr := root.children[childIdx];
+    && oldChildPtr.Some?
+
+    // Parent adds splitKey pivot; replaces child at childIdx with two children
+    && root'.ValidChildIndex(childIdx+1)  // obvious once we have replace1with2, but we're not there yet
+    && var leftChildPtr := root'.children[childIdx];
+    && var rightChildPtr := root'.children[childIdx+1];
+    && var childActiveRange := root.activeBufferRanges[childIdx];
+    && root' == root.(
+      pivotTable := InsertPivot(root.pivotTable, childIdx, splitKey),
+
+      // replace1with2 is just telling us about the structure of
+      // root'.children: the prefix and suffix are identical, and the new left
+      // & right child ptrs appear where childIdx once was. But it *doesn't*
+      // say anything about the value of leftChildPtr (resp. rightChildPtr),
+      // since we fetched those out of root'.children in the var statement
+      // above. That's a "clever" trick to leave nondeterminism that says we
+      // don't care what the actual values of those pointers are.
+      children := replace1with2(root.children, leftChildPtr, rightChildPtr, childIdx),
+      activeBufferRanges := replace1with2(root.activeBufferRanges, childActiveRange, childActiveRange, childIdx) // yea?
+
+      )
+
+    // Children get correspending slices
+    && leftChildPtr.Some?
+    && rightChildPtr.Some?
+
+    // TODO: we should be cleaning up pivot ranges, not buffers [revisit]
+
+    // && var oldChild := linked.diskView.Get(oldChildPtr);
+    // && var leftChild := linked'.diskView.Get(leftChildPtr);
+    // && var rightChild := linked'.diskView.Get(rightChildPtr);
+
+    // && leftChild == oldChild.ApplyFilter(Domain(root.pivotTable[childIdx-1], Element(splitKey)))
+    // && rightChild == oldChild.ApplyFilter(Domain(Element(splitKey), root.pivotTable[childIdx]))
+
+    // TODO(jonh): Say, ApplyFilter only affects buffers, but we also need to
+    // carve up the pivot tables and children! ...in PivotBetree, too.
+  }
+
+  predicate InternalSplit(v: Variables, v': Variables, lbl: TransitionLabel, step: Step)
+  {
+    // todo: rewrite
+    assume false; 
+    && v.WF()
+    && lbl.InternalLabel?
+    && step.InternalSplitStep?
+    && step.path.linked == v.linked
+    && step.path.Valid()
+    // // v && v' agree on everything down to Target()
+    // // && step.path.IsSubstitution(v.linked, v'.linked, [])
+    // // Target and Target' are related by a split operation
+    // && IsSplit(step.path.Target(), step.path.Target(), step.childIdx, step.splitKey)
+    // && v'.memtable == v.memtable  // UNCHANGED
+  }
+
+//   function InsertFlushReplacement(target: LinkedBetree, childIdx:nat, targetAddr: Address, targetChildAddr: Address) : (out: LinkedBetree)
+//     requires target.WF()
+//     requires target.HasRoot()
+//     requires target.Root().OccupiedChildIndex(childIdx)
+//   {
+//     var root := target.Root();
+//     var keepKeys := AllKeys() - root.ChildDomain(childIdx).KeySet();
+//     var keptBuffers := root.buffers.ApplyFilter(keepKeys);
+//     var movedBuffers := root.buffers.ApplyFilter(root.ChildDomain(childIdx).KeySet());
+//     // BetreeNode of the new child, to be stored at targetChildAddr in the diskview
+//     var subroot := target.diskView.Get(root.children[childIdx]);
+//     var subroot' := BetreeNode(subroot.buffers.PushBufferStack(movedBuffers), subroot.pivotTable, subroot.children);
+
+//     // BetreeNode of the new root, to be stored at targetAddr in the diskview
+//     var children' := root.children[childIdx := Pointer.Some(targetChildAddr)];
+//     var root' := BetreeNode(keptBuffers, root.pivotTable, children');
+    
+//     // The new diskview
+//     var dv' := DiskView.DiskView(target.diskView.entries[targetAddr := root'][targetChildAddr := subroot']); 
+//     LinkedBetree(Pointer.Some(targetAddr), dv')
+//   } 
+
+  // TODO: internal step for shifting the active buffer range, remove entries from the bufferstack
+
+  // makes no changes to the forest as a whole
+  // targetAddr: the node to flush, targetChildAddr: child with the latest update, pathAddrs: ancestor of flushed node
+  predicate InternalFlush(v: Variables, v': Variables, lbl: TransitionLabel, step: Step)
+  {
+    && v.WF()
+    && step.WF()
+    && lbl.InternalLabel?
+    && step.InternalFlushStep?
+    && step.path.linked == v.linked
+    && step.path.Valid()
+//     && step.path.Target().Root().OccupiedChildIndex(step.childIdx)  // the downstream child must exist
+//     // Subway Eat Fresh!
+//     && v.linked.diskView.IsFresh({step.targetAddr, step.targetChildAddr} + Set(step.pathAddrs))
+//     && v'.linked == step.path.Substitute( 
+//         InsertFlushReplacement(step.path.Target(), step.childIdx, step.targetAddr, step.targetChildAddr), 
+//         step.pathAddrs
+//     ).BuildTightTree()
+//     && v'.memtable == v.memtable  // UNCHANGED
+  }
+
+//   // target is the root node before it is compacted. 
+//   // InsertReplacement returns a LinkedBetree that has the diskview of target with replacement placed at
+//   // the replacementAddr
+//   function InsertCompactReplacement(target: LinkedBetree, compactedBuffers: BufferStack, replacementAddr: Address) : (out: LinkedBetree)
+//     requires target.WF()
+//     requires target.HasRoot()
+//     requires target.Root().buffers.Equivalent(compactedBuffers)
+//     ensures out.WF() 
+//   {
+//     var root := target.Root();
+//     var newRoot := BetreeNode(compactedBuffers, root.pivotTable, root.children);
+//     var newDiskView := DiskView.DiskView(target.diskView.entries[replacementAddr := newRoot]);
+//     LinkedBetree(GenericDisk.Pointer.Some(replacementAddr), newDiskView)
+//   }
+
+  // TODO: Compaction could result in removal of a tree, it is probably fine to use the full
+  // system state to decide this in the modeling and use a reference count in the implementation
+  // which refines to that, ref count should be tracked with this module and forest just takes a step to remove
+  // it's safe to do bc each step should maintain WF of variables which requires all buffers to be bounded 
+  // (are present in the tree)
+  predicate InternalCompact(v: Variables, v': Variables, lbl: TransitionLabel, step: Step)
+  {
+    && v.WF()
+    && step.WF()
+    && lbl.InternalLabel?
+    && step.InternalCompactStep?
+    && step.path.linked == v.linked
+    && step.path.Valid()
+//     && step.path.Target().Root().buffers.Equivalent(step.compactedBuffers)
+//     // Subway Eat Fresh!
+//     && v.linked.diskView.IsFresh({step.targetAddr} + Set(step.pathAddrs))
+//     && v'.linked == step.path.Substitute(
+//         InsertCompactReplacement(step.path.Target(), step.compactedBuffers, step.targetAddr), 
+//         step.pathAddrs
+//     ).BuildTightTree()
+//     && v'.memtable == v.memtable  // UNCHANGED
+  }
+
+//   // public:
+
+//   predicate Init(v: Variables, stampedBetree: StampedBetree)
+//   {
+//     && stampedBetree.value.WF()
+//     && stampedBetree.value.Acyclic()
+//     && v == Variables(EmptyMemtable(stampedBetree.seqEnd), stampedBetree.value)
+//   }
+
+  datatype Step =
+      QueryStep(receipt: QueryReceipt)
+    | PutStep()
+    | QueryEndLsnStep()
+    | FreezeAsStep()
+    | InternalFlushMemtableStep(branch: LB.LinkedBranch)
+    // newRootAddr is the new address allocated for the new root
+    | InternalGrowStep(newRootAddr: Address) 
+    | InternalSplitStep(path: Path, childIdx: nat, splitKey: Key)
+    // targetAddr is the fresh address at which new node is placed, and targetChildAddr is for the new child receiving the flush
+    // pathAddrs is the new addresses to place all its ancestors, used in substitution 
+    | InternalFlushStep(path: Path, childIdx: nat, targetAddr: Address, targetChildAddr: Address, pathAddrs: PathAddrs)
+    // targetAddr is the fresh address at which compactedNode is placed. pathAddrs is the new addresses to place all its ancestors
+    | InternalCompactStep(path: Path, compactedBuffers: BufferStack, targetAddr: Address, pathAddrs: PathAddrs)
+  {
+    predicate WF() {
+      match this {
+        case QueryStep(receipt) => receipt.Valid()
+        case InternalFlushMemtableStep(branch) =>
+          && branch.Acyclic()  // new branch must be acyclic
+
+//         case InternalSplitStep(path, childIdx, splitKey) => 
+//            && path.Valid()
+        case InternalFlushStep(_, _, targetAddr, targetChildAddr, pathAddrs) => 
+          && path.Valid()
+          && path.Target().Root().ValidChildIndex(childIdx)
+          && path.depth == |pathAddrs|
+          && SeqHasUniqueElems(pathAddrs) 
+          && {targetAddr, targetChildAddr} !! Set(pathAddrs)
+          && targetAddr != targetChildAddr
+//         case InternalCompactStep(path, compactedNode, targetAddr, pathAddrs) =>
+//           && path.Valid()
+//           && path.Target().Root().buffers.Equivalent(compactedBuffers)
+//           && path.depth == |pathAddrs|
+//           && SeqHasUniqueElems(pathAddrs) 
+//           && {targetAddr} !! Set(pathAddrs)
+        case _ => true
+      }
+    }
+  }
+
+//   predicate NextStep(v: Variables, v': Variables, lbl: TransitionLabel, step: Step)
+//   {
+//     match step {
+//       case QueryStep(receipt) => Query(v, v', lbl, receipt)
+//       case PutStep() => Put(v, v', lbl)
+//       case QueryEndLsnStep() => QueryEndLsn(v, v', lbl)
+//       case FreezeAsStep() => FreezeAs(v, v', lbl)
+//       case InternalGrowStep(_) => InternalGrow(v, v', lbl, step)
+//       case InternalSplitStep(_, _, _) => InternalSplit(v, v', lbl, step)
+//       case InternalFlushStep(_, _, _, _, _) => InternalFlush(v, v', lbl, step)
+//       case InternalCompactStep(_, _, _, _) => InternalCompact(v, v', lbl, step)
+//     }
+//   }
+
+//   predicate Next(v: Variables, v': Variables, lbl: TransitionLabel) {
+//     exists step: Step :: NextStep(v, v', lbl, step)
+//   }
+}
