Splinter/Betree/LinkedForest.i.dfy
@@ -1,0 +1,134 @@
+// Copyright 2018-2021 VMware, Inc., Microsoft Inc., Carnegie Mellon University, ETH Zurich, and University of Washington
+// SPDX-License-Identifier: BSD-2-Clause
+
+include "../Journal/GenericDisk.i.dfy"
+include "LinkedBranch.i.dfy"
+
+// Forest at linked layer 
+module LinkedForestMod {
+	import opened KeyType
+	import opened ValueMessage
+	import opened Sequences
+	import opened LinkedBranchMod
+  import D = GenericDisk
+
+	// Track the forest as trees and a single diskView
+	// We can construct LinkedBranch from each tree and the diskView
+	datatype LinkedForest = LinkedForest(trees: set<Address>, diskView: DiskView) 
+	{
+    // we currently do not require each b+tree to be disjoint from another 
+    // TODO: should we require each tree to be disjoint from another?
+    //       we could enforce that in addtree if we don't plan to init from a new one 
+		predicate WF() {
+			&& diskView.WF()
+			&& (forall root | root in trees :: diskView.ValidAddress(root))
+		}
+
+		predicate ValidTree(addr: Address)
+		{
+			addr in trees
+		}
+
+		function GetTree(addr: Address) : (branch: LinkedBranch)
+      requires WF()
+      requires ValidTree(addr)
+      ensures branch.WF()
+		{
+			LinkedBranch(addr, diskView)
+		}
+
+		function Query(key: Key, buffers: seq<Address>) : Message
+      requires WF()
+      requires (forall addr | addr in buffers :: ValidTree(addr))
+		{
+			if buffers == [] then Update(NopDelta())
+      else (
+				var tree := GetTree(Last(buffers));
+				Merge(Query(key, DropLast(buffers)), tree.Query(key))
+			)
+		}
+
+    predicate ValidRanking(ranking: D.Ranking) 
+      requires WF()
+    {
+      && diskView.ValidRanking(ranking)
+      && (forall root | root in trees :: root in ranking)
+    }
+
+    function TheRanking() : D.Ranking
+      requires Acyclic()
+    {
+      var out :| ValidRanking(out);
+      out
+    }
+
+    predicate Acyclic()
+    {
+      && WF()
+      && (exists ranking :: ValidRanking(ranking))
+    }
+	}
+  
+
+	datatype Step = AddTreeStep
+
+	datatype TransitionLabel =
+    AddTreeLabel(tree: LinkedBranch)
+  | RemoveTreeLabel(root: Address) // new diskview in step
+
+	datatype Variables = Variables(forest: LinkedForest) {
+		predicate WF() {
+			&& forest.WF()
+		}
+
+    function Addresses() : set<Address>
+		{
+			set addr | addr in forest.diskView.entries
+		}
+	}
+
+  // TODO: each tree is disjoint from another should be kept as an Inv
+  predicate AddTree(v: Variables, v': Variables, lbl: TransitionLabel) {
+    && lbl.AddTreeLabel?
+    && v.WF()
+    // new tree must be acyclic with fresh addresses
+    && lbl.tree.WF()
+    && lbl.tree.Acyclic()
+    && v.forest.diskView.IsFresh(lbl.tree.diskView.Addresses())
+    // updated forest
+    && v'.forest.trees == v.forest.trees + { lbl.tree.root }
+    && v'.forest.diskView == v.forest.diskView.MergeDisk(lbl.tree.diskView)
+    && v'.WF()
+  }
+
+  predicate RemoveTree(v: Variables, v': Variables, lbl: TransitionLabel) {
+    && lbl.RemoveTreeLabel?
+    && v.WF()
+    // new tree must be acyclic with fresh addresses
+    && lbl.root in v.forest.trees
+    // updated forest
+    // && v'.forest.trees == v.forest.trees + { lbl.tree.root }
+    // && v'.forest.diskView == v.forest.diskView.MergeDisk(lbl.tree.diskView) 
+    && v'.WF()
+  }
+
+	// public:
+
+  // TODO: might need to update to StampedLinkedForest
+  predicate Init(v: Variables) {
+    && v.WF()
+  }
+
+  predicate NextStep(v: Variables, v': Variables, lbl: TransitionLabel, step: Step)
+  {
+    match step {
+      case AddTreeStep() => AddTree(v, v', lbl)
+    }
+  }
+
+  predicate Next(v: Variables, v': Variables, lbl: TransitionLabel)
+  {
+    exists step :: NextStep(v, v', lbl, step)
+  }
+}
+
